rocq/PISA.ml
@@ -28,7 +28,7 @@ type instr =
 | INeg of reg
 | IExch of reg * reg
 | ISltx of reg * reg * reg
-| IOrx of reg * reg
+| IOrx of reg * reg * reg
 | IAndx of reg * reg * reg
 
 type code = instr list
@@ -61,16 +61,15 @@ let step i s =
           (if Z.ltb (s.regs rs) (s.regs rt) then 1 else 0))
         s.regs);
       mem = s.mem }
-  | IOrx (rd, rs) ->
+  | IOrx (rd, rs, rt) ->
     { regs =
-      (rupd rs 0 (rupd rd (Z.coq_lor (s.regs rd) (s.regs rs)) s.regs)); mem =
-      s.mem }
-  | IAndx (rd1, rd2, rs) ->
+      (rupd rd (Z.coq_lxor (s.regs rd) (Z.coq_lor (s.regs rs) (s.regs rt)))
+        s.regs);
+      mem = s.mem }
+  | IAndx (rd, rs, rt) ->
     { regs =
-      (rupd rd2 0
-        (rupd rd1
-          (Z.coq_lxor (s.regs rd1) (Z.coq_land (s.regs rd2) (s.regs rs)))
-          s.regs));
+      (rupd rd (Z.coq_lxor (s.regs rd) (Z.coq_land (s.regs rs) (s.regs rt)))
+        s.regs);
       mem = s.mem }
 
 (** val run : code -> state -> state **)
